Changed the interpretation of postconditions to enable refinement of the resource manager

Z_Machine.thy
@@ -8,15 +8,15 @@ text \<open> An operation is constructed from a precondition, update, and postco
   are parameterised. \<close>
 
 definition mk_zop :: "('a \<Rightarrow> 's \<Rightarrow> bool) \<Rightarrow> ('a \<Rightarrow> 's subst) \<Rightarrow> ('a \<Rightarrow> 's \<Rightarrow> bool) \<Rightarrow> ('a \<Rightarrow> ('e, 's) htree)" where
-"mk_zop P \<sigma> Q = (\<lambda> v. assert (P v) \<Zcomp> \<langle>\<sigma> v\<rangle>\<^sub>a \<Zcomp> assume (Q v))"
+"mk_zop P \<sigma> Q = (\<lambda> v. assume (P v) \<Zcomp> assert (Q v) \<Zcomp> \<langle>\<sigma> v\<rangle>\<^sub>a)"
 
 text \<open> An operation requires that precondition holds, and that following the update the postcondition(s)
   also hold. \<close>
 
-lemma wp_zop [wp, code_unfold]: "wp (mk_zop P \<sigma> Q v) b = [\<lambda> \<s>. P v \<s> \<and> (\<sigma> v \<dagger> [\<lambda> \<s>. Q v \<s> \<and> b \<s>]\<^sub>e) \<s>]\<^sub>e"
+lemma wp_zop [wp, code_unfold]: "wp (mk_zop P \<sigma> Q v) b = [\<lambda> \<s>. P v \<s> \<and> Q v \<s> \<and> (\<sigma> v \<dagger> [\<lambda> \<s>. b \<s>]\<^sub>e) \<s>]\<^sub>e"
   by (simp add: mk_zop_def wp)
 
-lemma wlp_zop [wp, code_unfold]: "wlp (mk_zop P \<sigma> Q v) b = [\<lambda> \<s>. P v \<s> \<longrightarrow> (\<sigma> v \<dagger> [\<lambda> \<s>. Q v \<s> \<longrightarrow> b \<s>]\<^sub>e) \<s>]\<^sub>e"
+lemma wlp_zop [wp, code_unfold]: "wlp (mk_zop P \<sigma> Q v) b = [\<lambda> \<s>. P v \<s> \<longrightarrow> Q v \<s> \<longrightarrow> (\<sigma> v \<dagger> [\<lambda> \<s>. b \<s>]\<^sub>e) \<s>]\<^sub>e"
   by (simp add: mk_zop_def wp)
 
 lemma itree_pre [dpre]: "itree_pre (mk_zop P \<sigma> Q v) = [\<lambda> \<s>. P v \<s>]\<^sub>e"
