examples/ResourceManager.thy
@@ -12,18 +12,18 @@ schema ResourceManager =
   where "free \<subseteq> res" "res \<subseteq> RES"
 
 record_default ResourceManager
-
+ 
 zoperation Allocate =
   over ResourceManager
   params r \<in> RES
-  pre "r \<in> free"
   update "[free \<leadsto> free - {r}]"
+  post "r \<in> free"
 
 zoperation Allocate\<^sub>1 =
   over ResourceManager
   params r \<in> RES
-  pre "r \<in> free \<and> r = Min free"
   update "[free \<leadsto> free - {r}]"
+  post "r \<in> free \<and> r = Min free"
 
 zoperation Deallocate =
   over ResourceManager
@@ -32,12 +32,12 @@ zoperation Deallocate =
   update "[free \<leadsto> free \<union> {r}]"
 
 lemma Allocate\<^sub>1_refines_Allocate: "Allocate r \<sqsubseteq> Allocate\<^sub>1 r"
-  apply (simp add: Allocate_def Allocate\<^sub>1_def input_in_rel assigns_rel refined_by_def input_in_pre assigns_pre seq_pre wp mk_zop_def)
-  oops
+  by (auto simp add: Allocate_def Allocate\<^sub>1_def input_in_rel dpre assigns_rel refined_by_def wp mk_zop_def
+      seq_rel assume_rel test_rel relcomp_unfold)
 
 zmachine ResourceManagerProc =
   init "[res \<leadsto> RES, free \<leadsto> RES]"
-  operations "Allocate" "Deallocate"
+  operations "Allocate\<^sub>1" "Deallocate"
 
 def_consts RES = "set (map integer_of_int [0..5])"
 
